lemma relating context to wlt

context.v
@@ -60,6 +60,16 @@ Definition chk_eq_wrt_ctx (ctx: ctx_t) (sv1 sv2: sstack_val) :=
   | _, _ => false
   end.
 
+Definition chk_lt_wrt_ctx (ctx: ctx_t) (sv1 sv2: sstack_val) :=
+  let imp_chkr := imp_checker_fun (ctx_imp_chkr ctx) in
+  let cs := ctx_cs ctx in
+  let ocl1 := sstack_val_to_cliteral sv1 in
+  let ocl2 := sstack_val_to_cliteral sv2 in
+  match ocl1, ocl2 with
+  | Some cl1, Some cl2 => imp_chkr cs  (C_LT cl1 cl2)
+  | _, _ => false
+  end.
+
 
 End Context.
 
