tests.v
@@ -125,7 +125,7 @@ Compute
   let b1 := str2block "MUL" in
   let b2 := str2block "POP POP PUSH1 0x0" in
   let init_state := (parse_init_state "2") in
-  let cs := [[C_EQ (C_VAR 1) (C_VAL 0)]] in
+  let cs := [[C_EQ (C_VAR 2) (C_VAL 0); C_EQ (C_VAR 2) (C_VAR 1)]] in
   match init_state with
   | Some (_,sst) =>
       (evm_eq_block_chkr_lazy
